ProgramLogic.v
@@ -5,7 +5,7 @@ Require Import Language.
 Require Export Logic.
 (* Require Import msl.msl_direct. *)
 
-Delimit Scope logic_scope with logic.
+(* Delimit Scope logic_scope with logic. *)
 
 Declare Module Semax : SEMAX.
 Import Semax.
